git/rebryant/model-counting/crat/prototype/ddnnf.py
@@ -4,6 +4,7 @@
 
 import sys
 import getopt
+import readwrite
 import schema
 
 # Format documentation: http://www.cril.univ-artois.fr/kc/d-DNNF-reasoner.html
@@ -45,17 +46,20 @@ import schema
 
 
 def usage(name):
-    print("Usage: %s [-h] [-v] [-p] -n N [-i FILE.cnf] [-p FILE.nnf] [-o FILE.crat]")
+    print("Usage: %s [-h] [-v] [-i FILE.cnf] [-n FILE.nnf] [-p FILE.crat]")
     print(" -h           Print this message")
     print(" -v           Add comments to files")
     print(" -i FILE.cnf  Input CNF")
-    print(" -p FILE.nnf  Input NNF")
-    print(" -o FILE.crat Output CRAT")
+    print(" -n FILE.nnf  Input NNF")
+    print(" -p FILE.crat Output CRAT")
 
-def trim(line):
-    while len(line) > 0 and line[-1] == '\n':
-        line = line[:-1]
-    return line
+class NnfException(Exception):
+
+    def __init__(self, value):
+        self.value = value
+
+    def __str__(self):
+        return "Nnf Exception: " + str(self.value)
 
 class NodeType:
     conjunction, disjunction, leaf, constant, ite = range(5)
@@ -70,28 +74,15 @@ class Node:
     ntype = None
     id = None
     children = []
-    litSet = set([])
-    varSet = set([])
+    # Corresponding schema node
+    snode = None
 
     def __init__(self, ntype, id, children):
         self.ntype = ntype
         self.id = id
         self.children = children
-        self.litSet = set([])
-        self.varSet = set([])
+        self.snode = None
         
-    def getVars(self):
-        if len(self.children) == 0:
-            return
-        self.litSet = set([])
-        self.varSet = set([])
-        for c in self.children:
-            self.litSet |= c.litSet
-            self.varSet |= c.varSet
-
-    def clone(self, nid):
-        return self
-
     def cstring(self):
         slist = ["N%d" % c.id for c in self.children]
         return '(' + ", ".join(slist) + ')'
@@ -100,7 +91,10 @@ class Node:
         return "N%d:%s%s" % (self.id, NodeType.name(self.ntype), self.cstring())
 
     def show(self):
-        print("%s  Lits = %s, Vars = %s" % (str(self), str(self.litSet), str(self.varSet)))
+        print(str(self))
+
+    def findLit(self, var):
+        return None
 
 class AndNode(Node):
     
@@ -114,12 +108,13 @@ class AndNode(Node):
             else:
                 nchildren.append(c)
         Node.__init__(self, NodeType.conjunction, id, lchildren + nchildren)
-        self.getVars()
         
-    def clone(self, nid):
-        nchildren = list(self.children)
-        nnode = AndNode(nid, nchildren)
-        return nnode
+    def findLit(self, var):
+        for c in self.children:
+            lit = c.findLit(var)
+            if lit is not None:
+                return lit
+        return None
 
 
 # Attempt optimizations
@@ -138,17 +133,13 @@ class OrNode(Node):
 
     def __init__(self, id, children, splitVar):
         # Put tchild first:
-        if -splitVar in children[0].litSet:
+        lit0 = children[0].findLit(splitVar)
+        if lit0 is None:
+            raise(NnfException("Couldn't find literal of variable %d in %s" % (splitVar, str(self))))
+        if lit0 == -splitVar:
             children.reverse()
         Node.__init__(self, NodeType.disjunction, id, children)
         self.splitVar = splitVar
-        self.getVars()
-
-    def clone(self, nid):
-        nchildren = list(self.children)
-        nnode = OrNode(nid, nchildren, self.splitVar)
-        return nnode
-
 
 def optOrNode(id, children, splitVar):
     if len(children) == 0:
@@ -163,14 +154,14 @@ class LeafNode(Node):
     def __init__(self, id, lit):
         Node.__init__(self, NodeType.leaf, id, [])
         self.lit = lit
-        self.litSet = set([lit])
-        self.varSet = set([abs(lit)])
-        
-    def clone(self, nid):
-        return LeafNode(self, nid, self.lit)
 
     def cstring(self):
         return '(' + str(self.lit) + ')'
+
+    def findLit(self, var):
+        if abs(self.lit) == var:
+            return self.lit
+        return None
 
 class ConstantNode(Node):
 
@@ -178,9 +169,6 @@ class ConstantNode(Node):
     def __init__(self, id, val):
         Node.__init__(self, NodeType.constant, id, [])
         self.val = val
-
-    def clone(self, nid):
-        return ConstantNode(self, nid, self.val)
 
     def cstring(self):
         return str(self.val)
@@ -192,9 +180,6 @@ class IteNode(Node):
     def __init__(self, id, children, splitVar):
         Node.__init__(self, NodeType.ite, id, children)
         self.splitVar = splitVar
-        self.getVars()
-        self.litSet |= set([splitVar, -splitVar])
-        self.varSet |= set([splitVar])
 
     def cstring(self):
         s = Node.cstring(self)
@@ -203,6 +188,9 @@ class IteNode(Node):
 class Nnf:
     verbose = False
     inputCount = 0
+    # Nodes are topologically ordered but their ids don't necessarily
+    # match position in the array, nor are they necessarily in
+    # ascending order
     nodes = []
 
     def __init__(self, verbose = False):
@@ -211,21 +199,19 @@ class Nnf:
 
     def nodeCount(self):
         count = 0
-        for node in self.nodes:
-            if node is not None:
-                count += 1
-        return count
+        return len(self.nodes)
 
     def read(self, infile):
         lineNumber = 0
         gotHeader = False
         ncount = 0
         ecount = 0
-        # Will perform some optimizations.  Prepare to have some get remapped
-        remap = {}
-        self.nodes = []
+        # Mapping from node id (given by order in file) to node
+        # Optimizations may cause some nodes to be reused
+        # but will maintain topological order
+        nodeDict = {}
         for line in infile:
-            line = trim(line)
+            line = readwrite.trim(line)
             lineNumber += 1
             fields = line.split()
             if len(fields) == 0:
@@ -255,11 +241,9 @@ class Nnf:
                 if var < 1 or var > self.inputCount:
                     print("Line #%d (%s).  Out of range literal" % (lineNumber, line))
                     return False
-                id = len(self.nodes)
+                id = len(nodeDict)
                 nnode = LeafNode(id, lit)
-                remap[id] = id
-                self.nodes.append(nnode)
-                
+                nodeDict[id] = nnode
             elif fields[0] == 'A':
                 try:
                     vals = [int(f) for f in fields[1:]]
@@ -269,76 +253,97 @@ class Nnf:
                 if len(vals) == 0 or vals[0] != len(vals)-1:
                     print("Line #%d (%s).  Incorrect number of arguments" % (lineNumber, line))
                     return False
-                id = len(self.nodes)
                 try:
-                    children = [self.nodes[remap[i]] for i in vals[1:]]
+                    children = [nodeDict[i] for i in vals[1:]]
                 except:
                     print("Line #%d (%s) Invalid argument specifier" % (lineNumber, line))
                     return False
+                id = len(nodeDict)
                 nnode = optAndNode(id, children)
-                nid = nnode.id
-                remap[id] = nid
-                if id == nid:
-                    self.nodes.append(nnode)
-                else:
-                    self.nodes.append(None)
+                nodeDict[id] = nnode
             elif fields[0] == 'O':
                 try:
                     vals = [int(f) for f in fields[1:]]
                 except:
                     print("Line #%d (%s).  Nonnumeric argument" % (lineNumber, line))
                     return False
-                if len(vals) != 2 and not (len(vals) == 4  and vals[2] != 2):
-                    print("Line #%d (%s).  Incorrect number of arguments" % (lineNumber, line))
+                if len(vals) < 2 or vals[1] != len(vals)-2:
+                    print("Line #%d (%s).  Incorrect number of arguments (%d)" % (lineNumber, line, len(vals)))
                     return False
                 nnode = None
                 splitVar = vals[0]
                 try:
-                    children = [self.nodes[remap[i]] for i in vals[2:]]
+                    children = [nodeDict[i] for i in vals[2:]]
                 except:
                     print("Line #%d (%s) Invalid argument specifier" % (lineNumber, line))
                     return False
-                id = len(self.nodes)
+                id = len(nodeDict)
                 nnode = optOrNode(id, children, splitVar)
-                nid = nnode.id
-                remap[id] = nid
-                if id == nid:
-                    self.nodes.append(nnode)
-                else:
-                    self.nodes.append(None)                
+                nodeDict[id] = nnode
         if not gotHeader:
             print("No header found")
             return False
+        # Compress into list
+        self.nodes = []
+        for id in sorted(nodeDict.keys()):
+            node = nodeDict[id]
+            if id == node.id:
+                self.nodes.append(node)
+            else:
+                key = node.key()
+                del self.uniqueTable[key]
+        root = nodeDict[len(nodeDict)-1]
+        self.topoSort(root)
         return True
+
+    # Perform topological sort of nodes, with root at end
+    # Eliminating any unreachable nodes
+    def topoSort(self, root):
+        nodeList = []
+        markSet = set([])
+        self.topoTraverse(root, nodeList, markSet)
+        self.nodes = nodeList
+        if self.verbose:
+            print("Topological sort:")
+            self.nodes.show()
+        
+    # Traverse nodes for topological sorting
+    def topoTraverse(self, root, nodeList, markSet):
+        if root.id in markSet:
+            return
+        markSet.add(root.id)
+        for c in root.children:
+            self.topoTraverse(c, nodeList, markSet)
+        nodeList.append(root)
 
     def show(self):
         for n in self.nodes:
-            if n is not None:
-                n.show()
+            n.show()
 
     def findIte(self):
-        newNodes = list(self.nodes)
+        idList = [node.id for node in self.nodes]
+        nodeDict = { node.id  : node for node in self.nodes }
+        # Mapping from old Id to new one for nodes that are replaced
         remap = {}
-        for id in range(len(self.nodes)):
-            node = self.nodes[id]
-            if node is None:
-                continue
-            node.children = [newNodes[remap[child.id]] for child in node.children]
+        for id in idList:
+            node = nodeDict[id]
+            node.children = [nodeDict[remap[child.id]] for child in node.children]
             if node.ntype != NodeType.disjunction:
                 id = node.id
                 remap[id] = id
                 continue
             splitVar = node.splitVar
-            tchild, fchild = newNodes[node.children[0].id], newNodes[node.children[1].id] 
+            tchild, fchild = nodeDict[node.children[0].id], nodeDict[node.children[1].id]
             tnode = None
             fnode = None
             if tchild.ntype == NodeType.leaf:
                 if tchild.lit != splitVar:
                     print("WARNING: Expected literal %d in ITE argument %s" % (splitVar, str(tchild)))
                 else:
-                    nid = len(newNodes)
+                    nid = len(nodeDict)
                     tnode = ConstantNode(nid, 1)
-                    newNodes.append(tnode)
+                    nodeDict[nid] = tnode
+                    remap[nid] = nid
             elif tchild.ntype == NodeType.conjunction:
                 nchildren = []
                 for c in tchild.children:
@@ -348,18 +353,19 @@ class Nnf:
                     tnode = nchildren[0]
                 elif len(nchildren) != len(tchild.children)-1:
                     print("WARNING: Didn't find literal %d in ITE argument %s" % (splitVar, str(tchild)))
-                    print("nchildren = %s" % str([str(c) for c in nchildren]))
                 else:
-                    nid = len(newNodes)
-                    tnode = AndNode(nid, newArgs)
-                    newNodes.append(tnode)
+                    nid = len(nodeDict)
+                    tnode = AndNode(nid, nchildren)
+                    nodeDict[nid] = tnode
+                    remap[nid] = nid
             if fchild.ntype == NodeType.leaf:
                 if fchild.lit != -splitVar:
                     print("WARNING: Expected literal %d in ITE argument %s" % (-splitVar, str(fchild)))
                 else:
-                    nid = len(newNodes)
-                    fnode = ConstantNode(nid, 0)
-                    newNodes.append(fnode)
+                    nid = len(nodeDict)
+                    fnode = ConstantNode(nid, 1)
+                    nodeDict[nid] = fnode
+                    remap[nid] = nid
             elif fchild.ntype == NodeType.conjunction:
                 nchildren = []
                 for c in fchild.children:
@@ -370,51 +376,62 @@ class Nnf:
                 elif len(nchildren) != len(fchild.children)-1:
                     print("WARNING: Didn't find literal %d in ITE argument %s" % (-splitVar, str(fchild)))
                 else:
-                    nid = len(newNodes)
-                    fnode = AndNode(nid, newArgs)
-                    newNodes.append(fnode)
+                    nid = len(nodeDict)
+                    fnode = AndNode(nid, nchildren)
+                    nodeDict[nid] = fnode
+                    remap[nid] = nid
             if tnode is not None and fnode is not None:
-                nid = len(newNodes)
+                nid = len(nodeDict)
                 nnode = IteNode(nid, [tnode, fnode], splitVar)
                 remap[nid] = nid
                 remap[node.id] = nid
-                newNodes.append(nnode)
-        rootId = remap[len(self.nodes)-1]
-        if rootId < len(newNodes)-1:
-            nid = len(newNodes)
-            nroot = newNodes[rootId].clone(nid)
-            newNodes.append(nroot)
-        return self.streamline(newNodes)
-
-    def streamline(self, nodes):
-        # Mark reachable nodes
-        marked = set([])
-        check = set([len(nodes)-1])
-        while len(check) > 0:
-            id = check.pop()
-            marked.add(id)
-            node = nodes[id]
-            for c in node.children:
-                cid = c.id
-                if cid not in marked and cid not in check:
-                    check.add(cid)
-
-        # Create new version of nodes
-        ndag = Nnf(self.verbose)
-        ndag.inputCount = self.inputCount
-        for node in nodes:
-            if node is None or len(ndag.nodes) not in marked:
-                ndag.nodes.append(None)
+                nodeDict[nid] = nnode
             else:
-                ndag.nodes.append(node)
-        return ndag
+                raise NnfException("Couldn't convert node %s into ITE" % (node))
+        # Compress into list
+        root = nodeDict[remap[self.nodes[-1].id]]
+        self.nodes = []
+        for id in sorted(nodeDict.keys()):
+            node = nodeDict[id]
+            if id == node.id:
+                self.nodes.append(node)
+        self.topoSort(root)
+
+    def schematize(self, clauseList, fname):
+        sch = schema.Schema(self.inputCount, clauseList, fname, verbLevel == 3 if self.verbose else 1)
+        for node in self.nodes:
+            if node is None:
+                continue
+            schildren = [child.snode for child in node.children]
+            if node.ntype == NodeType.constant:
+                node.snode = sch.leaf1 if node.val == 1 else sch.leaf0
+            elif node.ntype == NodeType.leaf:
+                var = abs(node.lit)
+                svar = sch.getVariable(var)
+                node.snode = svar if var > 0 else sch.addNegation(svar)
+            elif node.ntype == NodeType.conjunction:
+                # Build linear chain.   Keep literals at top
+                schildren.reverse()
+                nroot = schildren[0]
+                for c in schildren[1:]:
+                    nroot = sch.addConjunction(c, nroot)
+                node.snode = nroot
+            elif node.ntype == NodeType.disjunction:
+                node.snode = sch.addDisjunction(schildren[0], schildren[1])
+            elif node.ntype == NodeType.ite:
+                svar = sch.getVariable(node.splitVar)
+                node.snode = sch.addIte(svar, schildren[0], schildren[1])
+                # Label for proof generation
+                node.snode.iteVar = node.splitVar
+        sch.compress()
+        return sch
                 
 def run(name, args):
     verbose = False
     cnfName = None
     nnfName = None
     cratName = None
-    optlist, args = getopt.getopt(args, 'hvi:p:o:')
+    optlist, args = getopt.getopt(args, 'hvi:n:p:')
     for (opt, val) in optlist:
         if opt == '-h':
             usage(name)
@@ -423,16 +440,21 @@ def run(name, args):
             verbose = True
         elif opt == '-i':
             cnfName = val
-        elif opt == '-p':
+        elif opt == '-n':
             nnfName = val
-        elif opt == '-o':
+        elif opt == '-p':
             cratName = val
         else:
             print("Invalid option '%s'" % (opt))
             return
-#    if cnfName is None:
-#        print("Must give name of CNF file")
-#        return
+    if cnfName is None:
+        print("Must give name of CNF file")
+        return
+    try:
+        cnffile = open(cnfName, 'r')
+    except:
+        print("Couldn't open CNF file %s" % cnfName)
+    creader = readwrite.CnfReader(cnfName, verbLevel = 3 if verbose else 1)
     if nnfName is None:
         print("Must give name of NNF file")
         return
@@ -440,6 +462,7 @@ def run(name, args):
         nfile = open(nnfName, 'r')
     except:
         print("Couldn't open NNF file %s" % nnfName)
+        return
     
     dag = Nnf(verbose)
     if not dag.read(nfile):
@@ -448,13 +471,19 @@ def run(name, args):
         print("DAG has %d inputs, %d nodes" % (dag.inputCount, dag.nodeCount()))
     if verbose:
         dag.show()
-    dag = dag.findIte()
-    print("")
-    print("Streamlined DAG has %d nodes" % (dag.nodeCount()))
+        print("")
+        print("ITE extraction:")
+    dag.findIte()
+    print("Resulting DAG has %d nodes" % (dag.nodeCount()))
     if verbose:
         dag.show()
-    
-
+    if cratName is not None:
+        sch = dag.schematize(creader.clauses, cratName)
+        if verbose:
+            print("")
+            print("Generated schema has %d nodes:" % len(sch.nodes))
+            sch.show()
+        sch.doValidate()
 
 if __name__ == "__main__":
     run(sys.argv[0], sys.argv[1:])
