git/cruhland/lean4-axiomatic/Lean4Axiomatic/AbstractAlgebra.lean
@@ -43,16 +43,21 @@ For more information see `IdentityOn.ident` or
 [consult Wikipedia](https://en.wikipedia.org/wiki/Identity_element).
 
 **Named parameters**
-- `hand`: Indicates whether the property is left- or right-handed.
-- `α`: The `Sort` of the identity element and the parameters of the operation.
-- `e`: The identity element.
-- `f`: The binary operation that obeys the identity property with `e`.
+- `hand`:
+  Indicates whether the property is left- or right-handed.
+- `α`:
+  The `Sort` of the identity element and the parameters of the operation.
+- `e`:
+  The identity element. It's labeled as an `outParam` because it's useful to
+  have it be inferred in some contexts; see `InverseOn` for an example.
+- `f`:
+  The binary operation that obeys the identity property with `e`.
 
 **Class parameters**
 - `EqvOp α`: Necessary because the property expresses an equality on `α`.
 -/
 class IdentityOn
-    (hand : Hand) {α : Sort u} [EqvOp α] (e : α) (f : outParam (α → α → α))
+    (hand : Hand) {α : Sort u} [EqvOp α] (e : outParam α) (f : α → α → α)
     :=
   /--
   The left- or right-handed identity property of a distinguished element `e`
@@ -99,7 +104,7 @@ Convenience class for types, values, and operations that satisfy the full
 
 See `IdentityOn` for detailed documentation.
 -/
-class Identity {α : Sort u} [EqvOp α] (e : α) (f : outParam (α → α → α)) :=
+class Identity {α : Sort u} [EqvOp α] (e : outParam α) (f : α → α → α) :=
   identityL : IdentityOn Hand.L e f
   identityR : IdentityOn Hand.R e f
 
@@ -109,6 +114,10 @@ attribute [instance] Identity.identityR
 /--
 Derive the right-identity property from left-identity for operations `f`
 meeting certain conditions.
+
+**Intuition**: Both the left-handed and right-handed versions of the property
+equate an application of `f` to the same value. Thus if `f` is commutative, one
+version implies the other.
 
 **Named parameters**
 - `α`: The `Sort` of the identity element and the parameters of the operation.
@@ -128,6 +137,108 @@ def identityR_from_identityL
   intro (x : α)
   show f x e ≃ x
   exact Rel.trans AA.comm identL
+
+/--
+Class for types and operations that satisfy either the left- or right-handed
+inverse property.
+
+For more information see `InverseOn.inverse` or
+[consult Wikipedia](https://en.wikipedia.org/wiki/Inverse_element).
+
+**Named parameters**
+- `hand`: Indicates whether the property is left- or right-handed.
+- `α`: The `Sort` of the operations' parameters.
+- `e`: An identity element under the operation `f`.
+- `inv`: An operation that turns any `α` value into its inverse.
+- `f`: The binary operation that, with `inv`, obeys the inverse property.
+
+**Class parameters**
+- `EqvOp α`: Necessary because the property expresses an equality on `α`.
+- `IdentityOn hand e f`: Evidence that `e` is an identity element.
+-/
+class InverseOn
+    (hand : Hand) {α : Sort u} {e : α} (inv : outParam (α → α)) (f : α → α → α)
+    [EqvOp α] [IdentityOn hand e f]
+    :=
+  /--
+  The left- or right-handed inverse property of an inverse operation `inv` and
+  a binary operation `f` defined over a sort `α`.
+
+  The most well-known examples are additive and multiplicative inverses from
+  arithmetic. Integers are the simplest numbers to have additive inverses, via
+  negation; `a + (-a) ≃ (-a) + a ≃ 0` for all `a`. Similarly, rational numbers
+  are the simplest ones with multiplicative inverses, via reciprocation;
+  `q * q⁻¹ ≃ q⁻¹ * q ≃ 1` for all nonzero `q`.
+
+  **Named parameters**
+  - See `InverseOn` for the class parameters.
+  - `x`: The value that is combined (via `f`) with its own inverse.
+  -/
+  inverse {x : α} : hand.align f (inv x) x ≃ e
+
+export InverseOn (inverse)
+
+/--
+Convenience function for the left-handed inverse property.
+
+Can often resolve cases where type inference gets stuck when using the more
+general `inverse` function.
+
+See `InverseOn.inverse` for detailed documentation.
+-/
+abbrev inverseL := @inverse Hand.L
+
+/--
+Convenience function for the right-handed inverse property.
+
+Can often resolve cases where type inference gets stuck when using the more
+general `inverse` function.
+
+See `InverseOn.inverse` for detailed documentation.
+-/
+abbrev inverseR := @inverse Hand.R
+
+/--
+Convenience class for types and operations that satisfy the full (left- **and**
+right-handed) inverse property.
+
+See `InverseOn` for detailed documentation.
+-/
+class Inverse
+    {α : Sort u} {e : α} (inv : outParam (α → α)) (f : α → α → α)
+    [EqvOp α] [Identity e f] :=
+  inverseL : InverseOn Hand.L inv f
+  inverseR : InverseOn Hand.R inv f
+
+/--
+Derive the right-inverse property from left-inverse for operations `f`
+meeting certain conditions.
+
+**Intuition**: Both the left-handed and right-handed versions of the property
+equate an application of `f` to the same value. Thus if `f` is commutative, one
+version implies the other.
+
+**Named parameters**
+- `α`: The `Sort` of the operations' parameters.
+- `e`: An identity element under the operation `f`.
+- `inv`: An operation that turns any `α` value into its inverse.
+- `f`: The binary operation that, with `inv`, obeys the inverse property.
+
+**Class parameters**
+- `EqvOp α`: Necessary because the property expresses an equality on `α`.
+- `IdentityOn hand e f`: Evidence that `e` is an identity element.
+- `Commutative f`: Restriction on `f` that's required for the derivation.
+-/
+def inverseR_from_inverseL
+    {α : Sort u} {e : α} {inv : α → α} {f : α → α → α}
+    [EqvOp α] [Identity e f] [Commutative f]
+    : InverseOn Hand.L inv f → InverseOn Hand.R inv f
+    := by
+  intro _ -- Make left inverse available to instance search
+  apply InverseOn.mk
+  intro (x : α)
+  show f x (inv x) ≃ e
+  exact Rel.trans AA.comm inverseL
 
 /--
 Class for types and operations that satisfy either the left- or right-handed
